add most of an inductive definition for level checking
Signed-off-by: John Kastner <jkastner@amazon.com>

cedar-lean/Cedar/Thm/Validation/Levels/CheckLevel.lean
@@ -24,6 +24,297 @@ functions that do not need reason about the slicing functions.
 -/
 
 open Cedar.Validation
+open Cedar.Spec
+
+inductive EntityLit : TypedExpr → Prop where
+  | entity_lit {euid : EntityUID} {ty : CedarType} :
+    EntityLit (.lit (.entityUID euid) ty)
+  | ite_true {x₁ x₂ x₃ : TypedExpr} {ty : CedarType}
+    (hx₂ : EntityLit x₂) :
+    EntityLit (.ite x₁ x₂ x₃ ty)
+  | ite_false {x₁ x₂ x₃ : TypedExpr} {ty : CedarType}
+    (hx₃ : EntityLit x₃) :
+    EntityLit (.ite x₁ x₂ x₃ ty)
+  | get_attr {x₁ : TypedExpr} {a : Attr} {ty : CedarType}
+    (hx : EntityLit x₁) :
+    EntityLit (.getAttr x₁ a ty)
+  | get_tag {x₁ x₂ : TypedExpr} {ty : CedarType}
+    (hx₁ : EntityLit x₁) :
+    EntityLit (.binaryApp .getTag x₁ x₂ ty)
+  | record {attrs : List (Attr × TypedExpr)} {ty : CedarType} {a : Attr} {tx : TypedExpr}
+    (hx₁ : (a, tx) ∈ attrs)
+    (hx₂ : EntityLit tx) :
+    EntityLit (.record attrs ty)
+
+theorem not_entity_lit_spec (tx : TypedExpr) :
+  (notEntityLit tx = true) ↔ (¬ EntityLit tx)
+:= by
+  cases tx <;> try (
+    simp only [notEntityLit, true_iff]
+    intros h₁
+    cases h₁
+  )
+  case lit p _ =>
+    cases p <;> simp [notEntityLit]
+    case entityUID => constructor
+    all_goals {
+      intro h₁
+      cases h₁
+    }
+  case ite tx₁ tx₂ tx₃ _ =>
+    have ih₁ := not_entity_lit_spec tx₁
+    have ih₂ := not_entity_lit_spec tx₂
+    have ih₃ := not_entity_lit_spec tx₃
+    simp only [ih₁, ih₂, ih₃, notEntityLit, Bool.and_eq_true]
+    constructor
+    · intro ⟨hx₁, hx₂⟩ hite
+      cases hite <;> contradiction
+    · intro hite
+      constructor <;> (
+        intro h₁
+        apply hite
+      )
+      case left => exact EntityLit.ite_true h₁
+      case right => exact EntityLit.ite_false h₁
+  case binaryApp op tx₁ tx₂ _ =>
+    cases op <;> (
+      simp [notEntityLit]
+      try ( intro h₁ ; cases h₁ )
+    )
+    have ih₁ := not_entity_lit_spec tx₁
+    have ih₂ := not_entity_lit_spec tx₂
+    simp [ih₁, ih₂]
+    constructor
+    · intros h₁ h₂
+      cases h₂
+      contradiction
+    · intros h₁ h₂
+      apply h₁
+      exact EntityLit.get_tag h₂
+
+  case getAttr tx₁ _ _ =>
+    simp only [notEntityLit]
+    have ih₁ := not_entity_lit_spec tx₁
+    simp only [ih₁]
+    constructor
+    · intros h₁ h₂
+      cases h₂
+      contradiction
+    · intros h₁ h₂
+      apply h₁
+      exact EntityLit.get_attr h₂
+
+  case record attrs ty =>
+    simp [notEntityLit]
+    constructor
+    · intros h₁ h₂
+      cases h₂
+      rename_i a tx' hx₁ hx₂
+      specialize h₁ a tx' hx₂
+      have : sizeOf tx' < 1 + sizeOf attrs + sizeOf ty := by
+        have h₁ := List.sizeOf_lt_of_mem hx₂
+        rw [Prod.mk.sizeOf_spec] at h₁
+        omega
+      have ih := not_entity_lit_spec tx'
+      simp only [ih] at h₁
+      contradiction
+    · intro h₁ _ tx' h₂
+      have : sizeOf tx' < 1 + sizeOf attrs + sizeOf ty := by
+        have h₁ := List.sizeOf_lt_of_mem h₂
+        rw [Prod.mk.sizeOf_spec] at h₁
+        omega
+      have ih := not_entity_lit_spec tx'
+      simp only [ih]
+      intro h₃
+      apply h₁
+      exact EntityLit.record h₂ h₃
+
+inductive Level : TypedExpr → Nat → Prop where
+  | lit (p : Prim) (ty : CedarType) (n : Nat) :
+    Level (.lit p ty) n
+  | var (v : Var) (ty : CedarType) (n : Nat) :
+    Level (.var v ty) n
+  | ite (tx₁ tx₂ tx₃ : TypedExpr) (ty : CedarType) (n : Nat)
+    (hl₁ : Level tx₁ n)
+    (hl₂ : Level tx₂ n)
+    (hl₃ : Level tx₃ n) :
+    Level (.ite tx₁ tx₂ tx₃ ty) n
+  | and (tx₁ tx₂ : TypedExpr) (ty : CedarType) (n : Nat)
+    (hl₁ : Level tx₁ n)
+    (hl₂ : Level tx₂ n) :
+    Level (.and tx₁ tx₂ ty) n
+  | or (tx₁ tx₂ : TypedExpr) (ty : CedarType) (n : Nat)
+    (hl₁ : Level tx₁ n)
+    (hl₂ : Level tx₂ n) :
+    Level (.or tx₁ tx₂ ty) n
+  | unaryApp (op : UnaryOp) (tx₁ : TypedExpr) (ty : CedarType)
+    (hl₁ : Level tx₁ n) :
+    Level (.unaryApp op tx₁ ty) n
+  | mem (tx₁ tx₂ : TypedExpr) (ty : CedarType) (n : Nat)
+    (he : ¬ EntityLit tx₁)
+    (hl₁ : Level tx₁ n)
+    (hl₂ : Level tx₂ n.succ) :
+    Level (.binaryApp .mem tx₁ tx₂ ty) n.succ
+  | getTag (tx₁ tx₂ : TypedExpr) (ty : CedarType) (n : Nat)
+    (he : ¬ EntityLit tx₁)
+    (hl₁ : Level tx₁ n)
+    (hl₂ : Level tx₂ n.succ) :
+    Level (.binaryApp .getTag tx₁ tx₂ ty) n.succ
+  | hasTag (tx₁ tx₂ : TypedExpr) (ty : CedarType) (n : Nat)
+    (he : ¬ EntityLit tx₁)
+    (hl₁ : Level tx₁ n)
+    (hl₂ : Level tx₂ n.succ) :
+    Level (.binaryApp .hasTag tx₁ tx₂ ty) n.succ
+  | binaryApp (op : BinaryOp) (tx₁ tx₂ : TypedExpr) (ty : CedarType) (n : Nat)
+    (hop :
+      match op with
+      | .mem | .hasTag | .getTag => False
+      | _ => True)
+    (hl₁ : Level tx₁ n)
+    (hl₂ : Level tx₂ n) :
+    Level (.binaryApp op tx₁ tx₂ ty) n
+  | getAttr (tx₁ : TypedExpr) (a : Attr) (ty : CedarType) (n : Nat)
+    (he : ¬ EntityLit tx₁)
+    (hl₁ : Level tx₁ n) :
+    Level (.getAttr tx₁ a ty) n.succ
+  | hasAttr (tx₁ : TypedExpr) (a : Attr) (ty : CedarType) (n : Nat)
+    (he : ¬ EntityLit tx₁)
+    (hl₁ : Level tx₁ n) :
+    Level (.hasAttr tx₁ a ty) n.succ
+  | getAttrRecord (tx₁ : TypedExpr) (a : Attr) (ty : CedarType) (n : Nat)
+    (he : ¬ EntityLit tx₁)
+    (hl₁ : Level tx₁ n)
+    (hty :
+      match tx₁.typeOf with
+      | .record _ => True
+      | _ => False) :
+    Level (.getAttr tx₁ a ty) n.succ
+  | hasAttrRecord (tx₁ : TypedExpr) (a : Attr) (ty : CedarType) (n : Nat)
+    (he : ¬ EntityLit tx₁)
+    (hl₁ : Level tx₁ n)
+    (hty :
+      match tx₁.typeOf with
+      | .record _ => True
+      | _ => False) :
+    Level (.hasAttr tx₁ a ty) n.succ
+  | set (txs : List TypedExpr) (ty : CedarType) (n : Nat)
+    (hl : ∀ tx ∈ txs, Level tx n) :
+    Level (.set txs ty) n
+  | record (attrs : List (Attr × TypedExpr)) (ty : CedarType)
+    (hl : ∀ atx ∈ attrs, Level atx.snd n) :
+    Level (.record attrs ty) n
+  | call (xfn : ExtFun) (args : List TypedExpr) (ty : CedarType)
+    (hl : ∀ tx ∈ args, Level tx n) :
+    Level (.call cfn args ty) n
+
+theorem level_spec (tx : TypedExpr) (n : Nat):
+  (Level tx n ) ↔ (checkLevel tx n = true)
+:= by
+  cases tx
+  case lit =>
+    simp [checkLevel]
+    constructor
+  case var =>
+    simp [checkLevel]
+    constructor
+  case ite tx₁ tx₂ tx₃ _ =>
+    have ih₁ := level_spec tx₁ n
+    have ih₂ := level_spec tx₂ n
+    have ih₃ := level_spec tx₃ n
+    simp [checkLevel]
+    rw [←ih₁, ←ih₂, ←ih₃]
+    constructor
+    · intros h
+      cases h
+      (constructor <;> try constructor) <;> assumption
+    · intro ⟨⟨h₁, h₂⟩, h₃⟩
+      constructor <;> assumption
+
+  case or tx₁ tx₂ _ | and tx₁ tx₂ _ =>
+    have ih₁ := level_spec tx₁ n
+    have ih₂ := level_spec tx₂ n
+    simp [checkLevel]
+    rw [←ih₁, ←ih₂]
+    constructor
+    · intro h
+      cases h
+      constructor <;> assumption
+    · intro ⟨ h₁, h₂ ⟩
+      constructor <;> assumption
+
+  case unaryApp op tx₁ _ =>
+    have ih₁ := level_spec tx₁ n
+    simp [checkLevel]
+    rw [←ih₁]
+    constructor
+    · intro h
+      cases h
+      assumption
+    · intro h₁
+      constructor
+      assumption
+
+  case binaryApp op tx₁ tx₂ _ =>
+    cases op
+    case getTag | hasTag | mem =>
+      have ih₁ := level_spec tx₁ (n - 1)
+      have ih₂ := level_spec tx₂ n
+      simp [checkLevel]
+      rw [←ih₁, ←ih₂, not_entity_lit_spec]
+      constructor
+      · intro h
+        cases h
+        rename_i h₁ h₂ h₃
+        (constructor <;> try constructor <;> try constructor) <;> (
+          try simp
+          try assumption
+        )
+        contradiction
+      · intro ⟨ ⟨ ⟨ h₁, h₂⟩, h₃ ⟩ , h₄⟩
+        have ⟨ n', hn ⟩  : ∃ n' : Nat , n = n'.succ := by simp [h₂]
+        subst n
+        constructor <;> assumption
+    all_goals
+      have ih₁ := level_spec tx₁ n
+      have ih₂ := level_spec tx₂ n
+      simp [checkLevel]
+      rw [←ih₁, ←ih₂]
+      constructor
+      · intro h
+        cases h
+        rename_i h₁ h₂
+        simp [h₁, h₂]
+      · intro ⟨ h₁, h₂ ⟩
+        constructor <;> (
+          try simp
+          try assumption
+        )
+
+  case getAttr tx₁ a _  | hasAttr tx₁ a _  =>
+    simp [checkLevel]
+    split
+    · constructor
+      · intro h
+        cases h <;> simp [*] at *
+        rename_i n _ _
+        have ih₁ := level_spec tx₁ n
+        rw [←ih₁, not_entity_lit_spec]
+        constructor <;> assumption
+      · have ih₁ := level_spec tx₁ (n - 1)
+        simp
+        rw [←ih₁, not_entity_lit_spec]
+        intro h₁ h₂ h₃
+        have ⟨ n', hn ⟩  : ∃ n' : Nat , n = n'.succ := by simp [h₂]
+        subst n
+        constructor <;> assumption
+    · sorry
+
+  case set => sorry
+
+  case record => sorry
+
+  case call => sorry
+
 
 theorem check_level_checked_succ {e : TypedExpr} {n : Nat}
   (h₁ : checkLevel e n)
